SmtEquivChecker.v
@@ -18,22 +18,20 @@ Fixpoint symbolize_expr (e : expr) : smt_expr :=
   end.
 
 (* Function signature for Z3 equivalence checker *)
-Parameter sym_checker :  smt_expr -> smt_expr -> bool.
+Parameter sym_checker :  smt_expr -> smt_expr -> state -> bool.
+
+Definition smt_equiv_checker (e1 e2 : expr) (s : state) : bool := 
+  sym_checker (symbolize_expr e1) (symbolize_expr e2) s.
 
 (* Soundness of Z3: if the symbolic versions of 2 exprs are shown equivalent by z3, then the 2 exprs are equivalent *)
-Axiom sound_smt_checker : forall e1 e2 : expr, sym_checker (symbolize_expr e1) (symbolize_expr e2) = true -> forall s, aequiv e1 e2 s.
+Axiom sound_smt_checker : forall (e1 e2 : expr) (s : state), smt_equiv_checker e1 e2 s = true -> aequiv e1 e2 s.
+
+(* sym_checker satisfies reflexivity at the least; think we still need this. *)
+Axiom reflexive_sym_checker:  forall (e: smt_expr) (s: state), sym_checker e e s = true.
+
+(* If two exprs eval to the same thing, then the sym_checker will say true *)
+Axiom eval_sym_checker: forall (e1 e2: expr) (s: state), (eval_expr e1 s) = (eval_expr e2 s) -> smt_equiv_checker e1 e2 s = true.
+
 (* Can make it return Option<bool>, true, false, or error *)
 (* The most rigorous way of doing this is a syntax and semantics for SMT-LIB. Like the smt2 library for Lean. But may not buy you that much. *)
 (* Think about this as a converter from a DSL into SMTLIB. Rather than using a Z3 or bitvector tactic (like with the smt2 tactic z3). *)
-
-(* And prove it equivalent in the same way ... *)
-Definition smt_equiv_checker (e1 e2 : expr) (s : state) : bool := 
-  match e1, e2 with
-    | Constant n1, Constant n2 => Nat.eqb n1 n2
-    | Var name1, Var name2 => String.eqb name1 name2
-    | Plus e11 e12, Plus e21 e22 => sym_checker (SymPlus (symbolize_expr e11) (symbolize_expr e12))
-                                                (SymPlus (symbolize_expr e21) (symbolize_expr e22))
-    | Minus e11 e12, Minus e21 e22 => sym_checker (SymMinus (symbolize_expr e11) (symbolize_expr e12) )
-                                                  (SymMinus (symbolize_expr e21) (symbolize_expr e22))
-    | _, _ => false
-  end.
